@prefix qudt:  <http://qudt.org/schema/qudt#> .
@prefix ssd:   <http://www.w3.org/ns/sparql-service-description#> .
@prefix owl:   <http://www.w3.org/2002/07/owl#> .
@prefix xsd:   <http://www.w3.org/2001/XMLSchema#> .
@prefix skos:  <http://www.w3.org/2004/02/skos/core#> .
@prefix rdfs:  <http://www.w3.org/2000/01/rdf-schema#> .
@prefix qudt-unit: <http://qudt.org/vocab/unit#> .
@prefix qb:    <http://purl.org/linked-data/cube#> .
@prefix dgu:   <http://reference.data.gov.uk/def/reference/> .
@prefix ui:    <http://purl.org/linked-data/registry-ui#> .
@prefix dct:   <http://purl.org/dc/terms/> .
@prefix reg:   <http://purl.org/linked-data/registry#> .
@prefix qudt-quantity: <http://qudt.org/vocab/quantity#> .
@prefix grib2-parameter: <http://codes.wmo.int/grib2/schema/parameter/> .
@prefix api:   <http://purl.org/linked-data/api/vocab#> .
@prefix vann:  <http://purl.org/vocab/vann/> .
@prefix prov:  <http://www.w3.org/ns/prov#> .
@prefix foaf:  <http://xmlns.com/foaf/0.1/> .
@prefix common-unit: <http://codes.wmo.int/common/schema/unit/> .
@prefix cc:    <http://creativecommons.org/ns#> .
@prefix grib2-core: <http://codes.wmo.int/grib2/schema/core/> .
@prefix void:  <http://rdfs.org/ns/void#> .
@prefix version: <http://purl.org/linked-data/version#> .
@prefix bufr4-core: <http://codes.wmo.int/bufr4/schema/core/> .
@prefix rdf:   <http://www.w3.org/1999/02/22-rdf-syntax-ns#> .
@prefix ldp:   <http://www.w3.org/ns/ldp#> .
@prefix time:  <http://www.w3.org/2006/time#> .
@prefix qudt-dimension: <http://qudt.org/vocab/dimension#> .
@prefix vs:    <http://www.w3.org/2003/06/sw-vocab-status/ns#> .
@prefix common-core: <http://codes.wmo.int/common/schema/core/> .
@prefix dc:    <http://purl.org/dc/elements/1.1/> .

<http://codes.wmo.int/49-2/observable-property/AIRMETEvolvingConditionCollectionAnalysis>
        a                skos:Concept ;
        rdfs:label       "AIRMET Evolving Condition Collection Analysis"@en ;
        dct:description  "The set of physical properties evaluated as a result of an AIRMET, as specified in Technical Regulations, Volume II (WMO-No. 49): Meteorological Services for International Air Navigation."@en ;
        skos:notation    "AIRMETEvolvingConditionCollectionAnalysis" ;
        skos:prefLabel   "AIRMET Evolving Condition Collection Analysis" .

<http://codes.wmo.int/49-2/observable-property/SIGMETPositionCollectionAnalysis>
        a                skos:Concept ;
        rdfs:label       "SIGMET Position Collection Analysis"@en ;
        dct:description  "The set of locations where meteorological conditions exist to be reported in a SIGMET, as specified in Technical Regulations, Volume II (WMO-No. 49): Meteorological Services for International Air Navigation."@en ;
        skos:notation    "SIGMETPositionCollectionAnalysis" ;
        skos:prefLabel   "SIGMET Position CollectionAnalysis" .

<http://codes.wmo.int/49-2/observable-property/SIGMETEvolvingConditionCollectionAnalysis>
        a                skos:Concept ;
        rdfs:label       "SIGMET Evolving Condition Collection Analysis"@en ;
        dct:description  "The set of meteorological conditions  to be reported in a SIGMET, as specified in Technical Regulations, Volume II (WMO-No. 49): Meteorological Services for International Air Navigation."@en ;
        skos:notation    "SIGMETEvolvingConditionCollectionAnalysis" ;
        skos:prefLabel   "SIGMET Evolving Condition Collection Analysis" .

<http://codes.wmo.int/49-2/observable-property/MeteorologicalAerodromeTrendForecast>
        a                     skos:Concept ;
        rdfs:label            "Meteorological aerodrome trend forecast"@en ;
        dct:description       "The set of physical properties evaluated as a result of the trend forecast procedure of a routine or special aerodrome meteorological report (METAR or SPECI), as specified in the Technical Regulations (WMO-No. 49), Volume II – Meteorological Service for International Air Navigation."@en ;
        reg:delegationTarget  <http://codes.wmo.int/ui/resources/observableProperty_MeteorologicalAerodromeTrendForecast.xml> ;
        reg:forwardingCode    "200" ;
        reg:notation          "MeteorologicalAerodromeTrendForecast" ;
        skos:notation         "MeteorologicalAerodromeTrendForecast" ;
        skos:prefLabel        "Meteorological Aerodrome TrendForecast" .

<http://codes.wmo.int/49-2/observable-property/MeteorologicalAerodromeForecast>
        a                     skos:Concept ;
        rdfs:label            "Meteorological aerodrome forecast"@en ;
        dct:description       "The set of physical properties evaluated as a result of an aerodrome forecast (TAF), as specified in the Technical Regulations (WMO-No. 49), Volume II – Meteorological Service for International Air Navigation."@en ;
        reg:delegationTarget  <http://codes.wmo.int/ui/resources/observableProperty_MeteorologicalAerodromeForecast.xml> ;
        reg:forwardingCode    "200" ;
        reg:notation          "MeteorologicalAerodromeForecast" ;
        skos:notation         "MeteorologicalAerodromeForecast" ;
        skos:prefLabel        "Meteorological Aerodrome Forecast" .

<http://codes.wmo.int/49-2/observable-property/MeteorologicalAerodromeObservation>
        a                     skos:Concept ;
        rdfs:label            "Meteorological aerodrome observation"@en ;
        dct:description       "The set of physical properties evaluated as a result of the observation procedure of a routine or special aerodrome meteorological report (METAR or SPECI), as specified in the Technical Regulations (WMO-No. 49), Volume II – Meteorological Service for International Air Navigation."@en ;
        reg:delegationTarget  <http://codes.wmo.int/ui/resources/observableProperty_MeteorologicalAerodromeObservation.xml> ;
        reg:forwardingCode    "200" ;
        reg:notation          "MeteorologicalAerodromeObservation" ;
        skos:notation         "MeteorologicalAerodromeObservation" ;
        skos:prefLabel        "Meteorological Aerodrome Observation" .

<http://codes.wmo.int/49-2/observable-property>
        a                        skos:Collection , ldp:Container , reg:Register ;
        rdfs:label               "Code Table D-5: IWXXM observable properties" ;
        dct:description          "The items within this code table are composite observable properties that define the set of physical properties evaluated as a result of regulated procedures specified in Technical Regulations, Volume II (WMO-No. 49): Meteorological Services for International Air Navigation. These include aerodrome observation and forecast reports (e.g. METAR, SPECI and TAF)."@en ;
        dct:description          <http://codes.wmo.int/system/organization/wmo> ;
        dct:modified             "2017-11-23T11:08:18.808Z"^^xsd:dateTime ;
        reg:manager              <http://codes.wmo.int/system/organization/www-dm> ;
        reg:owner                <http://codes.wmo.int/system/organization/wmo> ;
        owl:versionInfo          5 ;
        skos:member              <http://codes.wmo.int/49-2/observable-property/MeteorologicalAerodromeTrendForecast> , <http://codes.wmo.int/49-2/observable-property/AIRMETEvolvingConditionCollectionAnalysis> , <http://codes.wmo.int/49-2/observable-property/MeteorologicalAerodromeForecast> , <http://codes.wmo.int/49-2/observable-property/MeteorologicalAerodromeObservation> , <http://codes.wmo.int/49-2/observable-property/SIGMETPositionCollectionAnalysis> , <http://codes.wmo.int/49-2/observable-property/SIGMETEvolvingConditionCollectionAnalysis> ;
        skos:notation            "D-5" ;
        ldp:membershipPredicate  skos:member .
